rustfrontend/Rustlight-base.v
@@ -33,6 +33,9 @@ Definition typeof_place p :=
 
 Inductive expr : Type :=
 | Econst_int: int -> type -> expr       (**r integer literal *)
+| Econst_float: float -> type -> expr   (**r double float literal *)
+| Econst_single: float32 -> type -> expr (**r single float literal *)
+| Econst_long: int64 -> type -> expr    (**r long integer literal *)
 | Eplace: usekind -> place -> type -> expr (**r use of a variable, the only lvalue expression *)
 | Eunop: unary_operation -> expr -> type -> expr  (**r unary operation *)
 | Ebinop: binary_operation -> expr -> expr -> type -> expr. (**r binary operation *)
@@ -40,24 +43,29 @@ Inductive expr : Type :=
 
 Definition typeof (e: expr) : type :=
   match e with
-  | Econst_int _ ty 
+  | Econst_int _ ty
+  | Econst_float _ ty
+  | Econst_single _ ty
+  | Econst_long _ ty                
   | Eplace _ _ ty
   | Eunop _ _ ty
   | Ebinop _ _ _ ty => ty
   end.
 
-
 Fixpoint to_ctype (ty: type) : option Ctypes.type :=
   match ty with
   | Tunit => Some Tvoid 
+  (* | Tbox _  => None *)
   | Tint sz si attr => Some (Ctypes.Tint sz si attr)
+  | Tlong si attr => Some (Ctypes.Tlong si attr)
+  | Tfloat fz attr => Some (Ctypes.Tfloat fz attr)
+  | Tstruct id attr => Some (Ctypes.Tstruct id attr)
+  | Tunion id attr => Some (Ctypes.Tunion id attr)
   | Tfunction tyl ty cc =>
       match to_ctype ty, to_ctypelist tyl with
       | Some ty, Some tyl => Some (Ctypes.Tfunction tyl ty cc)
       | _, _ => None
       end
-  | Tstruct id attr => Some (Ctypes.Tstruct id attr)
-  | Tunion id attr => Some (Ctypes.Tunion id attr)
   end
     
 with to_ctypelist (tyl: typelist) : option (Ctypes.typelist) :=
@@ -140,20 +148,6 @@ Definition own_env := PTree.t (list place).
 
 Definition empty_own_env : own_env := PTree.empty (list place).
 
-(** access mode for Rust types  *)
-Definition access_mode (ty: type) : mode :=
-  match ty with
-  | Tint I8 Signed _ => By_value Mint8signed
-  | Tint I8 Unsigned _ => By_value Mint8unsigned
-  | Tint I16 Signed _ => By_value Mint16signed
-  | Tint I16 Unsigned _ => By_value Mint16unsigned
-  | Tint I32 _ _ => By_value Mint32
-  | Tint IBool _ _ => By_value Mint8unsigned
-  | Tunit => By_nothing
-  | Tfunction _ _ _ => By_reference
-  | Tstruct _ _ => By_copy
-  | Tunion _ _ => By_copy
-end.
 
 (** Deference a location based on the type  *)
 
@@ -172,73 +166,83 @@ Inductive deref_loc (ty: type) (m: mem) (b: block) (ofs: ptrofs) : val -> Prop :
 
 (** Assign a value to a location  *)
 
-Inductive assign_loc (ty: type) (m: mem) (b: block) (ofs: ptrofs): val -> mem -> Prop :=
+Inductive assign_loc (ce: composite_env) (ty: type) (m: mem) (b: block) (ofs: ptrofs): val -> mem -> Prop :=
   | assign_loc_value: forall v chunk m',
       access_mode ty = By_value chunk ->
       Mem.storev chunk m (Vptr b ofs) v = Some m' ->
-      assign_loc ty m b ofs v m'
+      assign_loc ce ty m b ofs v m'
   | assign_loc_copy: forall b' ofs' bytes m',
       access_mode ty = By_copy ->
       (* consider a = b ( a and b are struct ) *)
       (* evaluate b is (Vptr b' ofs'), evaluate a is (b,ofs) *)      
-      (sizeof ty > 0 -> (alignof_blockcopy ty | Ptrofs.unsigned ofs')) ->
-      (sizeof ty > 0 -> (alignof_blockcopy ty | Ptrofs.unsigned ofs)) ->
+      (sizeof ce ty > 0 -> (alignof_blockcopy ce ty | Ptrofs.unsigned ofs')) ->
+      (sizeof ce ty > 0 -> (alignof_blockcopy ce ty | Ptrofs.unsigned ofs)) ->
       (* a and b are disjoint or equal *)
       b' <> b \/ Ptrofs.unsigned ofs' = Ptrofs.unsigned ofs
-             \/ Ptrofs.unsigned ofs' + sizeof ty <= Ptrofs.unsigned ofs
-             \/ Ptrofs.unsigned ofs + sizeof ty <= Ptrofs.unsigned ofs' ->
-      Mem.loadbytes m b' (Ptrofs.unsigned ofs') (sizeof ty) = Some bytes ->
+             \/ Ptrofs.unsigned ofs' + sizeof ce ty <= Ptrofs.unsigned ofs
+             \/ Ptrofs.unsigned ofs + sizeof ce ty <= Ptrofs.unsigned ofs' ->
+      Mem.loadbytes m b' (Ptrofs.unsigned ofs') (sizeof ce ty) = Some bytes ->
       Mem.storebytes m b (Ptrofs.unsigned ofs) bytes = Some m' ->
-      assign_loc ty m b ofs (Vptr b' ofs') m'.
+      assign_loc ce ty m b ofs (Vptr b' ofs') m'.
 
 (** Prefix of a place  *)
 
 Fixpoint is_prefix (p1 p2: place) : bool :=
   match p1, p2 with
   | Plocal id1 _, Plocal id2 _ => Pos.eqb id1 id2
-  | Plocal id1 _, Pderef p2' _ => is_prefix p1 p2'
-  | Pderef p1' _, Pderef p2' _ => is_prefix p1' p2'
+  | Plocal id1 _, Pfield p2' _ _ => is_prefix p1 p2'
+  | Pfield p1' _ _, Pfield p2' _ _ => is_prefix p1' p2'
+  (* | Plocal id1 _, Pderef p2' _ => is_prefix p1 p2' *)
+  (* | Pderef p1' _, Pderef p2' _ => is_prefix p1' p2' *)
   | _ ,_ => false
   end.
 
 Definition is_prefix_strict (p1 p2: place) : bool :=
   match p2 with
   | Plocal _ _ => false
-  | Pderef p2' _  => is_prefix p1 p2'
+  | Pfield p2' _ _ => is_prefix p1 p2'
+  (* | Pderef p2' _  => is_prefix p1 p2' *)
   end.
+
 
 Fixpoint local_of_place (p: place) :=
   match p with
   | Plocal id _ => id
-  | Pderef p' _ => local_of_place p'
+  | Pfield p' _ _ => local_of_place p'
   end.
 
+Definition is_sibling (p1 p2: place) : bool :=
+  Pos.eqb (local_of_place p1) (local_of_place p2)
+  && negb (is_prefix p1 p2 && is_prefix p2 p1).
 
-Definition erase_init_paths (ie: init_env) (p: place) : option init_env :=
+
+Definition remove_own' (own: own_env) (p: place) : option own_env :=
   let id := local_of_place p in
-  match PTree.get id ie with
-  | Some init_path =>
-      let erased := filter (fun p1 => negb (is_prefix p p1)) init_path in
-      Some (PTree.set id erased ie)
+  match PTree.get id own with
+  | Some own_path =>
+      let erased := filter (fun p1 => negb (is_prefix p p1)) own_path in
+      Some (PTree.set id erased own)
   | None => None
   end.
 
-Definition uninit_env (ie: init_env) (op: option place) : option init_env :=
+Definition remove_own (own: own_env) (op: option place) : option own_env :=
   match op with
   | Some p =>
       match typeof_place p with
-      | Tbox _ => erase_init_paths ie p
-      | Treference _ Mutable _ => erase_init_paths ie p
-      | _ => Some ie
+      (* we assume all the struct is not copyable *)
+      | Tstruct _ _ => remove_own' own p
+      (* | Tbox _ => remove_own' own p *)
+      (* | Treference _ Mutable _ => remove_own' own p *)
+      | _ => Some own
       end
-  | _ => Some ie
+  | _ => Some own
   end.
 
-Fixpoint uninit_env_list (ie: init_env) (opl: list (option place)) : option init_env :=
+Fixpoint remove_own_list (own: own_env) (opl: list (option place)) : option own_env :=
   match opl with
   | op::opl' =>
-      match uninit_env ie op with
-      | Some ie' => uninit_env_list ie' opl'
+      match remove_own own op with
+      | Some own' => remove_own_list own' opl'
       | None => None
       end
   | _ => None
@@ -247,7 +251,7 @@ Fixpoint uninit_env_list (ie: init_env) (opl: list (option place)) : option init
 
 (** Classify function (copy from Cop.v)  *)
 Inductive classify_fun_cases : Type :=
-  | fun_case_f (targs: typelist) (tres: type) (cc: calling_convention) (**r (pointer to) function *)
+| fun_case_f (targs: typelist) (tres: type) (cc: calling_convention) (**r (pointer to) function *)
 | fun_default.
 
 Definition classify_fun (ty: type) :=
@@ -260,6 +264,8 @@ Definition classify_fun (ty: type) :=
   
 Section SEMANTICS.
 
+Variable ge: genv.
+  
 (** ** Evaluation of expressions *)
 
 Section EXPR.
@@ -269,16 +275,29 @@ Variable m: mem.
 
 (* similar to eval_lvalue in Clight.v *)
 Inductive eval_place : place -> block -> ptrofs -> Prop :=
-| eval_Plocal: forall id l ty,
+| eval_Plocal: forall id b ty,
     (** TODO: there is no global variable, so we do not consider the
     gloabl environment *)
-    e!id = Some (l, ty) ->
-    eval_place (Plocal id ty) l Ptrofs.zero
-| eval_Pderef: forall p ty l ofs l' ofs',
-    eval_place p l ofs ->
-    deref_loc ty m l ofs (Vptr l' ofs') ->
-    eval_place (Pderef p ty) l' ofs'.
-
+    e!id = Some (b, ty) ->
+    eval_place (Plocal id ty) b Ptrofs.zero
+| eval_Pfield_struct: forall p ty b ofs delta id i co bf attr,
+    eval_place p b ofs ->
+    ty = Tstruct id attr ->
+    ge.(genv_cenv) ! id = Some co ->
+    field_offset ge i (co_members co) = OK (delta, bf) ->
+    eval_place (Pfield p i ty) b (Ptrofs.add ofs (Ptrofs.repr delta))
+| eval_Pfield_union: forall p ty b ofs delta id i co bf attr,
+    eval_place p b ofs ->
+    ty = Tunion id attr ->
+    ge.(genv_cenv) ! id = Some co ->
+    union_field_offset ge i (co_members co) = OK (delta, bf) ->
+    eval_place (Pfield p i ty) b (Ptrofs.add ofs (Ptrofs.repr delta)).
+    
+(* | eval_Pderef: forall p ty l ofs l' ofs', *)
+(*     eval_place p l ofs -> *)
+(*     deref_loc ty m l ofs (Vptr l' ofs') -> *)
+(*     eval_place (Pderef p ty) l' ofs'. *)
+ 
 (* eval_expr would produce a pair (v, op). Here [op] has type [Option
 place], if [op] is equal to [Some p], it means that this expression is
 a xvalue expression and the [p] is the place to be moved from.  *)
@@ -286,21 +305,27 @@ a xvalue expression and the [p] is the place to be moved from.  *)
 Inductive eval_expr : expr -> val -> option place ->  Prop :=
 | eval_Econst_int:   forall i ty,
     eval_expr (Econst_int i ty) (Vint i) None
+| eval_Econst_float:   forall f ty,
+    eval_expr (Econst_float f ty) (Vfloat f) None
+| eval_Econst_single:   forall f ty,
+    eval_expr (Econst_single f ty) (Vsingle f) None
+| eval_Econst_long:   forall i ty,
+    eval_expr (Econst_long i ty) (Vlong i) None
 | eval_Eunop:  forall op a ty v1 v aty mp,
     eval_expr a v1 mp ->
     (* Note that to_ctype Tbox = None *)
     to_ctype (typeof a) = Some aty ->
+    (** TODO: define a rust-specific sem_unary_operation  *)
     sem_unary_operation op v1 aty m = Some v ->
     eval_expr (Eunop op a ty) v mp
-(* undecided global environment *)
-(** TODO: remove the composite_env in sem_binary_operation *)
-(* | eval_Ebinop: forall op a1 a2 ty v1 v2 v ty1 ty2, *)
-(*     eval_expr a1 v1 -> *)
-(*     eval_expr a2 v2 -> *)
+(* | eval_Ebinop: forall op a1 a2 ty v1 v2 v ty1 ty2 mp1 mp2, *)
+(*     eval_expr a1 v1 mp1 -> *)
+(*     eval_expr a2 v2 mp2 -> *)
 (*     to_ctype (typeof a1) = Some ty1 -> *)
 (*     to_ctype (typeof a2) = Some ty2 -> *)
 (*     sem_binary_operation ge op v1 ty1 v2 ty2 m = Some v -> *)
-(*     eval_expr (Ebinop op a1 a2 ty) v. *)
+(*     (* For now, we do not return moved place in binary operation *) *)
+(*     eval_expr (Ebinop op a1 a2 ty) v None. *)
 | eval_Eplace_copy: forall p b ofs ty m v,
     eval_place p b ofs ->
     deref_loc ty m b ofs v ->
@@ -308,12 +333,6 @@ Inductive eval_expr : expr -> val -> option place ->  Prop :=
 | eval_Eplace_move: forall p b ofs ty m v,
     eval_place p b ofs ->
     deref_loc ty m b ofs v ->
-    (* Old design: clear the move environment in the evaluation of expression
-    (* (* Before move out a place, we should ensure that it is legal to move it *) *)
-    (* legal_move p = true -> *)
-    (* (* erase {p, *p, **p, ...} in the move env because after being *)
-    (* moved out, [p] no longer owns the location it points to *) *)
-    (* erase_move_paths me p = Some me' -> *) *)
     eval_expr (Eplace Move p ty) v (Some p)
 | eval_Eref: forall p b ofs mut ty,
     eval_place p b ofs ->
@@ -330,17 +349,17 @@ Inductive eval_exprlist : list expr -> typelist -> list val -> list (option plac
     eval_exprlist bl tyl vl opl ->
     eval_exprlist (a :: bl) (Tcons ty tyl) (v2 :: vl) (op :: opl).
 
-Inductive eval_boxexpr : boxexpr -> val -> option place -> mem -> Prop :=
-| eval_Rexpr: forall e v op,
-    eval_expr e v op ->
-    eval_boxexpr (Bexpr e) v op m
-| eval_Rbox: forall r v op m' m'' m''' b ty chunk,
-    typeof_boxexpr r = ty ->
-    eval_boxexpr r v op m' ->
-    Mem.alloc m' 0 (sizeof ty) = (m'', b) ->
-    access_mode ty = By_value chunk ->
-    Mem.store chunk m'' b 0 v = Some m''' ->
-    eval_boxexpr (Box r) (Vptr b Ptrofs.zero) op m'''.
+(* Inductive eval_boxexpr : boxexpr -> val -> option place -> mem -> Prop := *)
+(* | eval_Rexpr: forall e v op, *)
+(*     eval_expr e v op -> *)
+(*     eval_boxexpr (Bexpr e) v op m *)
+(* | eval_Rbox: forall r v op m' m'' m''' b ty chunk, *)
+(*     typeof_boxexpr r = ty -> *)
+(*     eval_boxexpr r v op m' -> *)
+(*     Mem.alloc m' 0 (sizeof ty) = (m'', b) -> *)
+(*     access_mode ty = By_value chunk -> *)
+(*     Mem.store chunk m'' b 0 v = Some m''' -> *)
+(*     eval_boxexpr (Box r) (Vptr b Ptrofs.zero) op m'''. *)
 
 
 End EXPR.
@@ -356,7 +375,7 @@ Inductive cont : Type :=
 | Klet: ident -> cont -> cont
 | Kloop1: statement -> statement -> cont -> cont
 | Kloop2: statement -> statement -> cont -> cont
-| Kcall: option ident  -> function -> env -> init_env -> cont -> cont.
+| Kcall: option ident  -> function -> env -> own_env -> cont -> cont.
 
 
 (** Pop continuation until a call or stop *)
@@ -386,7 +405,7 @@ Inductive state: Type :=
       (s: statement)
       (k: cont)
       (e: env)
-      (ie: init_env)
+      (ie: own_env)
       (m: mem) : state
   | Callstate
       (vf: val)
@@ -397,130 +416,66 @@ Inductive state: Type :=
       (res: val)
       (k: cont)
       (m: mem) : state.                          
-
-
-
-(** Drop the owned chain of the place [p] until it meets an unowned
-type or the place is not in the drop obligations. For example, if
-there is a chain "[p] -own-> [*p] -own-> [**p] -mut-> [***p] -own->
-[****p]", and the initialized env for [p] is {p, *p, **p, ***p}, then
-drop_place' would drop the location pointed by [p] and [*p] because
-[**p] is not an owned pointer. *)
-Inductive drop_place' (owned: list place) (p: place) (m: mem) (b: block) (ofs: ptrofs) : mem -> Prop :=
-| drop_base: forall ty,
-    typeof_place p = ty ->
-    (* It is not of type [Tbox] *)
-    not_owned_type ty = true ->
-    drop_place' owned p m b ofs m
-| drop_not_own: forall ty,
-    not_owned_type ty = false ->
-    (* Although p has type [Tbox], p has been moved out *)
-    not (In p owned) ->
-    drop_place' owned p m b ofs m
-| drop_box: forall ty ty' m' m'' b' ofs',
-    not_owned_type ty = false ->
-    deref_type ty = Some ty' ->
-    (* p owns the location it points to *)
-    In p owned ->
-    (* The contents in [p] is (Vptr b' ofs') *)
-    Mem.load Mptr m b (Ptrofs.signed ofs) = Some (Vptr b' ofs') ->
-    drop_place' owned (Pderef p ty') m b' ofs' m' ->
-    (* Free the contents in (b',ofs') *)
-    Mem.free m' b' (Ptrofs.signed ofs') ((Ptrofs.signed ofs') + sizeof ty') = Some m'' ->
-    drop_place' owned p m b ofs m''.
-
-(** Free {*p, **p ,... } according to me  *)
-Inductive drop_place (e: env) (ie: init_env) (p: place) (m: mem) : mem -> Prop :=
-| drop_gen: forall b ofs m' id owned,
-    eval_place e m p b ofs ->
-    local_of_place p = id ->
-    PTree.get id ie = Some owned ->
-    drop_place' owned p m b ofs m' ->
-    drop_place e ie p m m'.
-
-Inductive drop_place_list (e: env) (ie: init_env) (m: mem) : list place -> mem -> Prop :=
-| drop_place_list_base:
-    drop_place_list e ie m nil m
-| drop_place_list_cons: forall p lp m' m'',
-    drop_place e ie p m m' ->
-    drop_place_list e ie m' lp m'' ->
-    drop_place_list e ie m (p::lp) m''.
-  
        
 
-(* Variable function_entry: function -> list val -> mem -> env -> mvenv -> mem -> Prop. *)
-
-(** Transition relation *)
-
-(** [TODEL] If a place [p] owns a location through box, it has the drop
-obligations. In other words, if [p] has type [Tbox] then [p] in its
-drop obligation list. A special case is the mutable reference, if [p]
-has type [&mut T], then we should not terminate the obligation
-generation, instead we should generate the obligations for [*p] (i.e.,
-skip [p]). For example, if [p:&mut Box<i32> = &mut x] and [*p =
-new_box], we should drop *p. Note that when x goes out of scope, it
-would drop the [new_box]. *)
-(* Fixpoint drop_obligations (p: place) (ty: type) : list place := *)
-(*   match ty with *)
-(*   | Tbox ty' => *)
-(*       let deref := Pderef p ty' in *)
-(*       p :: drop_obligations deref ty' *)
-(*   | Treference ty' Mutable _ => *)
-(*       let deref := Pderef p ty' in *)
-(*       drop_obligations deref ty' *)
-(*   | _ => nil *)
-(*   end. *)
-
-Fixpoint init_path (p: place) (ty: type) : list place :=
+Fixpoint own_path (ce: composite_env) (p: place) (ty: type) : list place :=
   match ty with
-  | Tbox ty' =>
-      let deref := Pderef p ty' in
-      p :: init_path deref ty'
-  | Treference ty' Mutable _ =>
-      let deref := Pderef p ty' in
-      p :: init_path deref ty'
+  (* | Tbox ty' => *)
+  (*     let deref := Pderef p ty' in *)
+  (*     p :: init_path deref ty' *)
+  (* | Treference ty' Mutable _ => *)
+  (*     let deref := Pderef p ty' in *)
+  (*     p :: init_path deref ty' *)
+  | Tstruct id attr =>
+      let co := ce ! id in
+      match co with
+      | Some co =>
+          let fields := map (fun m => match m with | Member_plain id ty => (Pfield p id ty) end) co.(co_members) in
+          p :: fields
+      | _ => p :: nil
+      end
+  (* For now, we do not consider Tunion as own type *)
   | _ => nil
   end.
   
 
 
-
 (** Allocate memory blocks for function parameters and build the local environment and move environment  *)
-Inductive alloc_variables: env -> init_env -> mem ->
-                           list (ident * type) ->
-                           env -> init_env -> mem -> Prop :=
+Inductive alloc_variables (ce: composite_env) : env -> own_env -> mem ->
+                                                list (ident * type) ->
+                                                env -> own_env -> mem -> Prop :=
 | alloc_variables_nil:
-  forall e ie m,
-    alloc_variables e ie m nil e ie m
+  forall e own m,
+    alloc_variables ce e own m nil e own m
 | alloc_variables_cons:
-  forall e ie m id ty vars m1 b1 m2 e2 ie2 drops,
-    Mem.alloc m 0 (sizeof ty) = (m1, b1) ->
+  forall e own m id ty vars m1 b1 m2 e2 own1 drops,
+    Mem.alloc m 0 (sizeof ce ty) = (m1, b1) ->
     (* get the initialized path based on ty *)
-    init_path (Plocal id ty) ty = drops ->
-    alloc_variables (PTree.set id (b1, ty) e) (PTree.set id drops ie) m1 vars e2 ie2 m2 ->
-    alloc_variables e ie m ((id, ty) :: vars) e2 ie2 m2.
+    own_path ce (Plocal id ty) ty = drops ->
+    alloc_variables ce (PTree.set id (b1, ty) e) (PTree.set id drops own) m1 vars e2 own1 m2 ->
+    alloc_variables ce e own m ((id, ty) :: vars) e2 own1 m2.
 
 (** Assign the values to the memory blocks of the function parameters  *)
-Inductive bind_parameters (e: env):
+Inductive bind_parameters (ce: composite_env) (e: env):
                            mem -> list (ident * type) -> list val ->
                            mem -> Prop :=
   | bind_parameters_nil:
       forall m,
-      bind_parameters e m nil nil m
+      bind_parameters ce e m nil nil m
   | bind_paranmeters_cons:
       forall m id ty params v1 vl b m1 m2,
       PTree.get id e = Some(b, ty) ->
-      assign_loc ty m b Ptrofs.zero v1 m1 ->
-      bind_parameters e m1 params vl m2 ->
-      bind_parameters e m ((id, ty) :: params) (v1 :: vl) m2.
+      assign_loc ce ty m b Ptrofs.zero v1 m1 ->
+      bind_parameters ce e m1 params vl m2 ->
+      bind_parameters ce e m ((id, ty) :: params) (v1 :: vl) m2.
 
 (** Return the list of blocks in the codomain of [e], with low and high bounds. *)
 
-Definition block_of_binding (id_b_ty: ident * (block * type)) :=
-  match id_b_ty with (id, (b, ty)) => (b, 0, sizeof ty) end.
+Definition block_of_binding (ce: composite_env) (id_b_ty: ident * (block * type)) :=
+  match id_b_ty with (id, (b, ty)) => (b, 0, sizeof ce ty) end.
 
-Definition blocks_of_env (e: env) : list (block * Z * Z) :=
-  List.map block_of_binding (PTree.elements e).
+Definition blocks_of_env (ce: composite_env) (e: env) : list (block * Z * Z) :=
+  List.map (block_of_binding ce) (PTree.elements e).
 
 (** Return the list of places in local environment  *)
 
@@ -531,39 +486,35 @@ Definition places_of_env (e:env) : list place :=
   List.map place_of_binding (PTree.elements e).
                                   
 
-
 (** Function entry semantics: the key is to instantiate the move environments  *)
-Inductive function_entry (ge: genv) (f: function) (vargs: list val) (m: mem) (e: env) (ie: init_env) (m': mem) : Prop :=
+Inductive function_entry (ge: genv) (ce: composite_env) (f: function) (vargs: list val) (m: mem) (e: env) (own: own_env) (m': mem) : Prop :=
 | function_entry_intro: forall m1,
     list_norepet (var_names f.(fn_params)) ->
-    alloc_variables empty_env empty_init_env m f.(fn_params) e ie m1 ->
-    bind_parameters e m1 f.(fn_params) vargs m' ->
-    function_entry ge f vargs m e ie m'.
- 
-Section WITH_GE.
+    alloc_variables ce empty_env empty_own_env m f.(fn_params) e own m1 ->
+    bind_parameters ce e m1 f.(fn_params) vargs m' ->
+    function_entry ge ce f vargs m e own m'.
 
-Variable ge: genv.
 
-Inductive step: state -> trace -> state -> Prop :=
+Inductive step : state -> trace -> state -> Prop :=
 
-| step_assign: forall f be p op k le ie ie' ie'' m1 m2 m3 m4 b ofs ty v,
+| step_assign: forall f be p op k le own own' own'' m1 m2 m3 m4 b ofs ty v,
     typeof_place p = ty ->
-    typeof_boxexpr be = ty ->             (* for now, just forbid type casting *)
+    typeof be = ty ->             (* for now, just forbid type casting *)
     (* get the location of the place *)
-    eval_place le m1 p b ofs ->
+    eval_place le p b ofs ->
     (* evaluate the boxexpr, return the value and the moved place (optional) *)
-    eval_boxexpr le m1 be v op m2 ->
+    eval_expr le m1 be v op ->
     (* update the initialized environment based on [op] *)
-    uninit_env ie op = Some ie' ->
+    remove_own own op = Some own' ->
     (* drop the successors of p (i.e., *p, **p, ...). If ty is not
     owned type, drop_place has no effect. We must first update the me
     and then drop p, consider [ *p=move *p ] *)
-    drop_place le ie' p m2 m3 ->
+    (* drop_place le ie' p m2 m3 -> *)
     (* update the init env for p *)
-    PTree.set (local_of_place p) (init_path p (typeof_place p)) ie' = ie'' ->    
+    PTree.set (local_of_place p) (own_path ge p (typeof_place p)) own' = own'' ->    
     (* assign to p  *)    
     assign_loc ty m3 b ofs v m4 ->
-    step (State f (Sassign p be) k le ie m1) E0 (State f Sskip k le ie'' m4)
+    step (State f (Sassign p be) k le own m1) E0 (State f Sskip k le own'' m4)
          
 | step_let: forall f be op v ty id ie1 ie2 ie3 m1 m2 m3 m4 le1 le2 b k stmt,
     typeof_boxexpr be = ty ->
